common/SmallstepLinkingSafe.v
@@ -10,10 +10,28 @@ Require Import Invariant.
 
 (** Module safety : similar to the preservation of invariant in LTS *)
 
-(* efinition safe {liA liB st} (L: lts liA liB st) (s: st) : Prop := *)
- (*  (exists r, final_state L s r) *)
- (*  \/ (exists q, at_external L s q) *)
- (*  \/ (exists t, exists s', Step L s t s'). *)
+(* Safety should be irrelevant to the trace *)
+Definition safe {liA liB st} (L: lts liA liB st) (s: st) : Prop :=
+  forall s' t,
+    Star L s t s' ->
+    (exists r, final_state L s' r)
+    \/ (exists q, at_external L s' q)
+    \/ (exists t, exists s'', Step L s' t s'').
+
+Lemma safe_implies {liA liB st} (L: lts liA liB st) s:
+  safe L s ->
+  Smallstep.safe L s.
+Proof.
+  intros. red. intros.
+  eapply H. eauto.
+Qed.
+
+Lemma star_safe:
+  forall {liA liB st} (L: lts liA liB st) s s' t,
+  Star L s t s' -> safe L s -> safe L s'.
+Proof.
+  intros; red; intros. eapply H0. eapply star_trans; eauto.
+Qed.
 
 Definition not_stuck {liA liB st} (L: lts liA liB st) (s: st) : Prop :=
   (exists r, final_state L s r)
@@ -474,9 +492,14 @@ Lemma lts_safe_reachable_safe {li1 li2 S} se (L: lts li1 li2 S) I1 I2 w : forall
     lts_safe se L I1 I2 not_stuck w ->
     reachable I1 I2 L w s ->
     safe L s.
-Admitted.
-
-
+Proof.
+  intros.
+  red. intros.
+  eapply reachable_safe in H.
+  2: { eapply star_reachable; eauto. }
+  eauto.
+Qed.
+   
 (** Unfinished: The following code is a more general module_safety
 property which supports different invariant in incoming side and
 outgoing side *)
@@ -568,6 +591,258 @@ Admitted.
 
 (** End of this unfinished general compose_safety  *)
 
+Record bsim_invariant {li1 li2} (cc: callconv li1 li2) (I1: invariant li1) (I2: invariant li2) : Type :=
+  {
+    (* incoming_query2 and outgoing_query2 are used to establish
+    match_states between reachable states *)
+    incoming_query2: forall w2 se2,
+      symtbl_inv I2 w2 se2 ->
+      exists ccw w1 se1,
+        match_senv cc ccw se1 se2
+        /\ symtbl_inv I1 w1 se1
+        /\ (forall q2, query_inv I2 w2 q2 ->
+                 exists q1, match_query cc ccw q1 q2
+                       /\ query_inv I1 w1 q1
+                       /\ (* outgoing_reply1 is embedded here because it is
+                            stated in w2. It is used to establish progress
+                            properties *)
+                         forall r1 r2, reply_inv I1 w1 r1 ->
+                                  match_reply cc ccw r1 r2 ->
+                                  reply_inv I2 w2 r2);
+
+    (** So ugly! used to establish reachable_match *)
+    outgoing_query2: forall w1 w2 ccw q1 q2 r2,
+      query_inv I2 w2 q2 ->
+      match_query cc ccw q1 q2 ->
+      query_inv I1 w1 q1 ->
+      (* incoming_reply2 is embedded here *)
+      reply_inv I2 w2 r2 ->
+      exists r1, reply_inv I1 w1 r1 /\
+              match_reply cc ccw r1 r2;
+
+    (* outgoing_query1 and incoming_reply1 are used to establish
+    progress properties *)
+    outgoing_query1: forall w1 ccw q1 q2 se1 se2,
+      query_inv I1 w1 q1 ->
+      symtbl_inv I1 w1 se1 ->
+      match_query cc ccw q1 q2 ->
+      match_senv cc ccw se1 se2 ->
+      exists w2 , query_inv I2 w2 q2
+                /\ symtbl_inv I2 w2 se2
+                /\ (* why here is incoming_reply2 ??? to establish after_external progress *)
+                  forall r2, reply_inv I2 w2 r2 ->
+                        exists r1, reply_inv I1 w1 r1
+                              /\ match_reply cc ccw r1 r2;    
+    
+  }.
+
+
+(* What is this? *)
+Record preservable_inv {li1 li2} (cc: callconv li1 li2) (I1: invariant li1) : Type :=
+  { query_inv_preserve: forall w1 wcc wcc' q1 q2 q1',
+      query_inv I1 w1 q1 ->
+      match_query cc wcc q1 q2 ->
+      match_query cc wcc' q1' q2 ->
+      query_inv I1 w1 q1';
+  }.
+
+
+(* Using constructive target invariant to prove safe preservatin *)
+Section SAFETY_PRESERVATION.
+
+Context {li1 li2} (cc: callconv li1 li2).
+Context (L1: semantics li1 li1) (L2: semantics li2 li2).
+Context (I1 : invariant li1) (I2: invariant li2).
+
+Hypothesis (INVPRE: preservable_inv cc I1).
+
+Section BSIM.
+  
+Context se1 se2 wcc (w1: inv_world I1) bsim_index bsim_order bsim_match_states
+  (BSIMP: bsim_properties cc cc se1 se2 wcc (L1 se1) (L2 se2) bsim_index bsim_order (bsim_match_states se1 se2 wcc)).
+
+Context (MENV: match_senv cc wcc se1 se2).
+
+(* Hypothesis (INQ: forall q1' wcc' wA', *)
+(*                match_query cc wcc' q1' q2 -> *)
+(*                query_inv IA wA' q1 -> *)
+(*                query_inv IA wA' q1'). *)
+
+
+Let match_states := bsim_match_states se1 se2 wcc.
+
+Lemma bsim_simulation_star_under_lts_safe: forall s2 t s2',
+    Star (L2 se2) s2 t s2' ->
+    forall i s1, safe (L1 se1) s1 ->
+            match_states i s1 s2 ->
+            exists i', exists s1', Star (L1 se1) s1 t s1' /\ match_states i' s1' s2'.
+Proof.
+  induction 1; intros.
+  exists i; exists s1; split; auto. apply star_refl.
+  exploit (@bsim_simulation li1); eauto.
+  eapply safe_implies. auto.
+  intros [i' [s2' [A B]]].
+  exploit IHstar. 2: eauto.
+  destruct A.
+  eapply star_safe. eapply plus_star; eauto. auto.
+  destruct H4. eapply star_safe; eauto.  
+  intros [i'' [s2'' [C D]]].
+  exists i''; exists s2''; split; auto. eapply star_trans; eauto.
+  intuition auto. apply plus_star; auto.
+Qed.
+
+
+Lemma bsim_reachable_match: forall s2,
+    reachable (invcc_out I1 cc) (invcc_in I1 cc) (L2 se2) (w1, wcc) s2 ->
+    lts_safe se1 (L1 se1) I1 I1 not_stuck w1 ->
+    exists s1 i, reachable I1 I1 (L1 se1) w1 s1
+            /\ bsim_match_states se1 se2 wcc i s1 s2.
+Proof.
+  induction 1; intros SAFE.
+  (* initial_reach *)
+  - destruct WT as (q1 & MQ & QINV1). 
+    assert (VQ1: valid_query (L1 se1) q1 = true).
+    { erewrite <- bsim_match_valid_query; eauto. }
+    (* initial_match *)
+    edestruct @bsim_match_initial_states as [EXIST MATCH]; eauto.
+    (* L1 is not stuck in initial states *)
+    exploit (@initial_progress li1); eauto.
+    intros (s1 & INIT1).
+    exploit EXIST; eauto. intros INIT2.
+    exploit MATCH. eapply INIT1. eapply INIT.
+    intros (s1' & INIT1' & (i & MATCH')).
+    (* prove bsim_simulation_star *)
+    exploit bsim_simulation_star_under_lts_safe; eauto.
+    eapply lts_safe_reachable_safe; eauto.
+    eapply initial_reach; eauto. eapply star_refl.
+    intros (i' & s1'' & STAR1 & MATCH'').
+    exists s1'', i'. split.
+    eapply star_reachable. eauto.
+    eapply initial_reach; eauto.
+    eapply star_refl. auto.
+  (* external reach *)
+  - exploit IHreachable; eauto.
+    intros (s1' & i1 & REACH1 & MATCH1).
+    (* external_simulation *)
+    exploit (@bsim_match_external li1); eauto.
+    eapply safe_implies.
+    eapply lts_safe_reachable_safe; eauto.
+    intros (wcc' & s1'' & q1 & STAR1 & ATEXT1 & MQ1 & MSE1 & AFEXT1).
+    eapply star_reachable in STAR1; eauto.
+    (* external_progress in L1 *)
+    exploit (@external_progress li1); eauto.
+    intros (w1' & SYM1 & QINV1 & AFEXT2).
+    (* get the well-typed query and reply *)
+    exploit WTR; eauto. intros (r1 & MQ & RINV1).
+    (* construct the matched after_external state *)
+    exploit AFEXT1; eauto.
+    intros [EXIST MATCH].
+    exploit AFEXT2; eauto.
+    intros (s' & AFEXT1'').
+    exploit MATCH; eauto.
+    intros (s1'0 & AFEXT'0 & (i & MATCH')).
+    (* prove bsim_simulation_star *)
+    exploit bsim_simulation_star_under_lts_safe; eauto.
+    eapply lts_safe_reachable_safe; eauto.
+    eapply external_reach; eauto. eapply star_refl.
+    intros (i' & s1''0 & STAR2 & MATCH'').
+    exists s1''0, i'. split; auto.
+    eapply star_reachable. eauto.
+    eapply external_reach; eauto.
+    eapply star_refl.
+Qed.
+
+End BSIM.
+  
+Lemma module_safety_preservation:  
+  module_safe L1 I1 I1 not_stuck ->
+  backward_simulation cc cc L1 L2 ->
+  module_safe L2 (invcc_out I1 cc) (invcc_in I1 cc) not_stuck.
+Proof.
+  intros SAFE [BSIM].
+  red. intros se2 VSE2.
+  red. intros (w1, wcc) SYM2.
+  (* construct se1 *)
+  destruct SYM2 as (se1 & SYM1 & MSE).
+  (* generalize (@incoming_query2 li1 li2 cc I1 I2 BSIM_INV _ _ SYM2). *)
+  (* intros (wcc & w1 & se1 & MSE & SYM1 & INQ).    *)
+  assert (VSE1: Genv.valid_for (skel L1) se1).
+  { eapply match_senv_valid_for; eauto.
+    erewrite bsim_skel; eauto. }
+  exploit SAFE; eauto.
+  intros LTSSAFE1.
+  destruct BSIM.
+  generalize (bsim_lts se1 se2 wcc MSE VSE1). intros BSIMP.
+  econstructor.
+  (* reachable_safe *)
+  - intros s2 REACH2.
+    exploit bsim_reachable_match; eauto.
+    intros (s1 & i & REACH1 & MATCH).
+    (* s1 is not_stuck *)
+    exploit (@reachable_safe li1); eauto.
+    (** NOTSTUCK1 is useless because one step in target program may
+    correspond to multiple steps in source program, so the property of
+    only one step not stuck in source program is not useful *)
+    intros NOTSTUCK1.
+    (* We use bsim_progress! *)
+    eapply bsim_progress; eauto.
+    eapply safe_implies.
+    eapply lts_safe_reachable_safe; eauto.
+  (* initial progress *)
+  - intros q2 VQ QINV2.
+    destruct QINV2 as (q1 & QINV1 & MQ).
+    (* exploit INQ; eauto. *)
+    (* intros (q1 & MQ & QINV1 & FINAL). *)
+    assert (VQ1: valid_query (L1 se1) q1 = true).
+    { erewrite <- bsim_match_valid_query; eauto. }
+    (* initial_match *)
+    edestruct @bsim_match_initial_states as [EXIST MATCH]; eauto.
+    (* L1 is not stuck in initial states *)
+    exploit (@initial_progress li1); eauto.
+    intros (s1 & INIT). eapply EXIST. eauto.
+  (* external_progress *)
+  - intros s2 q2 REACH2 ATEXT2.
+    exploit bsim_reachable_match; eauto.
+    intros (s1 & i & REACH1 & MATCH).
+    (* external_simulation *)
+    exploit (@bsim_match_external li1); eauto.
+    eapply safe_implies.
+    eapply lts_safe_reachable_safe; eauto.
+    intros (wcc' & s1'' & q1 & STAR1 & ATEXT1 & MQ1 & MSE1 & AFEXT1).
+    eapply star_reachable in STAR1; eauto.
+    (* q1 is well-typed *)
+    exploit (@external_progress li1);eauto.
+    intros (w1' & SYM1' & QINV1 & AFEXT1').
+    (* construct w2 and q2 *)
+    exists w1'.
+    (* generalize (@outgoing_query1 li1 li2 cc I1 I2 BSIM_INV  _ _ _ _ _ _ QINV1 SYM1' MQ1 MSE1). *)
+    (* intros (w2' & se2' & QINV2 & AFEXT2'). *)
+    (* exists w2'. *) repeat apply conj; auto.
+    simpl. exists se1, wcc'. auto.
+    simpl. intros. eapply query_inv_preserve; eauto.
+    simpl. intros r2 QINV2.
+    exploit QINV2; eauto. intros (r1 & MR & RINV1).
+    exploit AFEXT1'; eauto. intros (s1''' & A).
+    exploit AFEXT1; eauto. intros [EXIST MATCH1].
+    eapply EXIST. eauto.
+  (* final progress *)
+  - intros s r REACH2 FS2.
+    simpl.
+    exploit bsim_reachable_match; eauto.
+    intros (s1 & i & REACH1 & MATCH).
+    (* final_simulation *)
+    edestruct (@bsim_match_final_states li1) as (s1' & r1 & STAR & FS1 & MR); eauto.
+    eapply safe_implies.
+    eapply lts_safe_reachable_safe; eauto.
+    exists r1. split; eauto.
+    eapply final_progress. eauto.
+    eapply star_reachable; eauto.
+    auto.
+Qed.
+    
+    
+End SAFETY_PRESERVATION.
+
 
 (* similar to ccref *)
 Record bsim_invariant {li1 li2} (cc: callconv li1 li2) (I1: invariant li1) (I2: invariant li2) : Type :=
@@ -598,7 +873,7 @@ Record bsim_invariant {li1 li2} (cc: callconv li1 li2) (I1: invariant li1) (I2: 
       reply_inv I2 w2 r2 ->
       exists r1, reply_inv I1 w1 r1 /\
               match_reply cc ccw r1 r2;
-    
+
     (* outgoing_query1 and incoming_reply1 are used to establish
     progress properties *)
     outgoing_query1: forall w1 ccw q1 q2 se1 se2,
@@ -627,76 +902,6 @@ Context (I1 : invariant li1) (I2: invariant li2).
 
 Hypothesis BSIM_INV: bsim_invariant cc I1 I2.
 
-(* Lemma module_safety_preservation_se se1 se2 ccw: *)
-(*   match_senv cc ccw se1 se2 -> *)
-(*   module_safe_se L1 I1 I1 safe se1 -> *)
-(*   backward_simulation cc cc L1 L2 -> *)
-(*   module_safe_se L2 I2 I2 safe se2. *)
-(* Proof. *)
-  (* (** Test2  *) *)
-  (* intros MSENV SAFE [BSIM]. *)
-  (* destruct BSIM as [index order match_states SKEL PROP WF]. *)
-  (* red. intros w2 VSE2 SINV2. *)
-  (* (* set (safe' (l: lts li2 li2 (state L2)) s := *) *)
-  (* (*        exists w1: inv_world I1, *) *)
-  (* (*          safe l s /\ *) *)
-  (* (*          symtbl_inv I1 w1 se1 /\ *) *)
-  (* (*          forall r1, *) *)
-  (* (*            reply_inv I1 w1 r1 -> *) *)
-  (* (*            exists r2, reply_inv I2 w2 r2). *) *)
-
-  (* (* cut (lts_safe se2 (L2 se2) I2 I2 safe' w2). *) *)
-  (* split. *)
-  (* - admit. *)
-  (* (* initial_safe *) *)
-  (* - intros q2 VQ2 QINV2. *)
-  (*   destruct (inv_initial _ _ _ BSIM_INV w2 se1 se2 ccw q2 SINV2 MSENV QINV2) as (w1 & q1 & SINV1 & QINV1 & MQ). *)
-  (*   assert (VSE1: Genv.valid_for (skel L1) se1). *)
-  (*   (** TODO: we need the invert of match_senv_valid_for  *) *)
-  (*   admit. *)
-  (*   assert (VQ1: valid_query (L1 se1) q1 = true). *)
-  (*   { erewrite <- bsim_match_valid_query. eauto. *)
-  (*     eapply PROP. eauto. *)
-  (*     auto. auto. } *)
-  (*   edestruct (initial_safe _ _ _ _ _ _ (SAFE w1 VSE1 SINV1) q1 VQ1 QINV1) as ((s1 & INIT1) & INIT1').  *)
-  (*   edestruct @bsim_match_initial_states as [EXIST MATCH]; eauto. *)
-  (*   split. *)
-  (*   + eapply EXIST. eauto. *)
-  (*   + intros s2 INIT2. *)
-  (*     (** use bsim_progress *) *)
-  (*     exploit MATCH; eauto. *)
-  (*     intros (s1' & INIT1'' & (idx & MST)). *)
-  (*     (* show s1' is safe *) *)
-  (*     exploit INIT1'. eapply INIT1''. intros SAFES1'. *)
-  (*     (** TODO: use safe s1' and step_safe to prove smallstep.safe s1' *) *)
-  (*     eapply bsim_progress; eauto. *)
-  (*     admit. *)
-  (* - intros s2 q2 REACH2 EXTERN2. *)
-  (*   (** TODO: how to prove there is a reachable state s1 and s1 simulates s2*) *)
-  (*   assert (A: exists s1 idx, reachable (L1 se1) s1 /\ match_states se1 se2 ccw idx s1 s2). *)
-  (*   admit. *)
-  (*   destruct A as (s1 & idx & REACH1 & MST). *)
-    
-    
-  (** Test1  *)
-  (* intros MSENV SAFE BSIM. *)
-  (* inv BSIM. rename X into BSIM. *)
-  (* red. intros w2 VSE2 INV2. *)
-  (* generalize (inv_match_symtbl cc I1 I2 BSIM_INV w2 se1 se2 ccw INV2 MSENV). *)
-  (* intros (w1 & INV1). *)
-  (* assert (VSE1: Genv.valid_for (skel L1) se1). *)
-  (* (** TODO: use match_senv to prove it but match_senv does not guarantee the *)
-  (* backward valid_for? *)   *)
-  (* admit.  *)
-  (* exploit SAFE; eauto. *)
-  (* intros LTSSAFE1. *)
-  (* (* use bsim_lts *) *)
-  (* inv BSIM. generalize (bsim_lts se1 se2 ccw MSENV VSE1). *)
-  (* intros bsim_prop. inv bsim_prop. *)
-(* Admitted. *)
-
-
-
 Section BSIM.
   
 Context se1 se2 wcc (w1: inv_world I1) (w2: inv_world I2) bsim_index bsim_order bsim_match_states            
@@ -712,13 +917,29 @@ Hypothesis (INQ: forall q2 : query li2,
                    (forall (r1 : reply li1) (r2 : reply li2),
                        reply_inv I1 w1 r1 -> match_reply cc wcc r1 r2 -> reply_inv I2 w2 r2)).
 
+
 Let match_states := bsim_match_states se1 se2 wcc.
 
 Lemma bsim_simulation_star_under_lts_safe: forall s2 t s2',
     Star (L2 se2) s2 t s2' ->
-    forall i s1, match_states i s1 s2 ->
+    forall i s1, safe (L1 se1) s1 ->
+            match_states i s1 s2 ->
             exists i', exists s1', Star (L1 se1) s1 t s1' /\ match_states i' s1' s2'.
-Admitted.
+Proof.
+  induction 1; intros.
+  exists i; exists s1; split; auto. apply star_refl.
+  exploit (@bsim_simulation li1); eauto.
+  eapply safe_implies. auto.
+  intros [i' [s2' [A B]]].
+  exploit IHstar. 2: eauto.
+  destruct A.
+  eapply star_safe. eapply plus_star; eauto. auto.
+  destruct H4. eapply star_safe; eauto.  
+  intros [i'' [s2'' [C D]]].
+  exists i''; exists s2''; split; auto. eapply star_trans; eauto.
+  intuition auto. apply plus_star; auto.
+Qed.
+
 
 Lemma bsim_reachable_match: forall s2,
     reachable I2 I2 (L2 se2) w2 s2 ->
@@ -744,6 +965,8 @@ Proof.
     intros (s1' & INIT1' & (i & MATCH')).
     (* prove bsim_simulation_star *)
     exploit bsim_simulation_star_under_lts_safe; eauto.
+    eapply lts_safe_reachable_safe; eauto.
+    eapply initial_reach; eauto. eapply star_refl.
     intros (i' & s1'' & STAR1 & MATCH'').
     exists s1'', i'. split.
     eapply star_reachable. eauto.
@@ -754,6 +977,7 @@ Proof.
     intros (s1' & i1 & REACH1 & MATCH1 & FINAL).
     (* external_simulation *)
     exploit (@bsim_match_external li1); eauto.
+    eapply safe_implies.
     eapply lts_safe_reachable_safe; eauto.
     intros (wcc' & s1'' & q1 & STAR1 & ATEXT1 & MQ1 & MSE1 & AFEXT1).
     eapply star_reachable in STAR1; eauto.
@@ -773,6 +997,8 @@ Proof.
     intros (s1'0 & AFEXT'0 & (i & MATCH')).
     (* prove bsim_simulation_star *)
     exploit bsim_simulation_star_under_lts_safe; eauto.
+    eapply lts_safe_reachable_safe; eauto.
+    eapply external_reach; eauto. eapply star_refl.
     intros (i' & s1''0 & STAR2 & MATCH'').
     exists s1''0, i'. split; auto.
     eapply star_reachable. eauto.
@@ -814,6 +1040,7 @@ Proof.
     intros NOTSTUCK1.
     (* We use bsim_progress! *)
     eapply bsim_progress; eauto.
+    eapply safe_implies.
     eapply lts_safe_reachable_safe; eauto.
   (* initial progress *)
   - intros q2 VQ QINV2.
@@ -832,6 +1059,7 @@ Proof.
     intros (s1 & i & REACH1 & MATCH & FINAL).
     (* external_simulation *)
     exploit (@bsim_match_external li1); eauto.
+    eapply safe_implies.
     eapply lts_safe_reachable_safe; eauto.
     intros (wcc' & s1'' & q1 & STAR1 & ATEXT1 & MQ1 & MSE1 & AFEXT1).
     eapply star_reachable in STAR1; eauto.
@@ -856,6 +1084,7 @@ Proof.
     intros (s1 & i & REACH1 & MATCH & FINAL).
     (* final_simulation *)
     edestruct (@bsim_match_final_states li1) as (s1' & r1 & STAR & FS1 & MR); eauto.
+    eapply safe_implies.
     eapply lts_safe_reachable_safe; eauto.
     eapply FINAL; eauto.
     eapply final_progress. eauto.
